\[
   x^2 + 2x + 6 = -3x
\]

`swap-sides-with + right`

\[
   x^2 + 2x + 6 + 3x = 0
\]

`make x^2 xx`

\[
   xx + 2x + 6 + 3x = 0
\]

`factor-out x from {left 0, left 1, left 3}`

\[
   x(x+2+3) + 6 = 0
\]

`back 1`

\[
   xx + 2x + 6 + 3x = 0
\]


`factor-out x from {left 0, left 1}`

\[
   x(x + 2) + 6 + 3x = 0
\]

`factor-out 3 from {left 1, left 2}`

\[
   x(x+2) + 3(2 + x) = 0
\]

`factor-out x+2 from {left 0, left 1}`

\[
   (x+2)(x+3) = 0
\]

`split 0 produce`

\[
   (1) x+2 = 0          (2) x+3 = 0
\]

`1 isolate x && 2 isolate x`

\[
   (1) x = -2           (2) x = -3
\]
